Prove all modifies lemmas except modifies_loc_unused_in

ulib/FStar.MG2.fst
@@ -94,6 +94,12 @@ type cls (aloc: Type) : Type = | Cls:
     Lemma
     ((x `aloc_used_in` h /\ y `aloc_unused_in` h) ==> x `aloc_disjoint` y)
   )) ->
+  (aloc_used_in_or_unused_in: (
+    (x: aloc) ->
+    (h: HS.mem) ->
+    Lemma
+    (x `aloc_used_in` h \/ x `aloc_unused_in` h)
+  )) ->
   (aloc_used_in_includes: (
     (greater: aloc) ->
     (lesser: aloc) ->
@@ -122,7 +128,8 @@ type cls (aloc: Type) : Type = | Cls:
 type loc (#aloc: Type) (c: cls aloc) = (s: GSet.set aloc { forall (greater lesser: aloc) . {:pattern (greater `GSet.mem` s); (greater `c.aloc_includes` lesser)} greater `GSet.mem` s /\ greater `c.aloc_includes` lesser ==> lesser `GSet.mem` s })
 
 let loc_of_aloc #al (#c: cls al) (b: al) : GTot (loc c) =
-  admit()
+  Classical.forall_intro_3 (fun x y -> Classical.move_requires (c.aloc_includes_trans x y));
+  GSet.comprehend (fun x -> FStar.StrongExcludedMiddle.strong_excluded_middle (b `c.aloc_includes` x))
 
 let loc_none #al (#c: cls al) : Tot (loc c) =
   GSet.empty
@@ -146,7 +153,7 @@ let loc_disjoint_none_r
   (s: loc c)
 : Lemma
   (ensures (loc_disjoint s loc_none)) =
-  admit()
+  ()
 
 let loc_disjoint_union_r
   (#aloc: Type) (#c: cls aloc)
@@ -154,7 +161,7 @@ let loc_disjoint_union_r
 : Lemma
   (requires (loc_disjoint s s1 /\ loc_disjoint s s2))
   (ensures (loc_disjoint s (loc_union s1 s2))) =
-  admit()
+  ()
 
 let loc_disjoint_includes
   (#aloc: Type) (#c: cls aloc)
@@ -162,7 +169,7 @@ let loc_disjoint_includes
 : Lemma
   (requires (loc_includes p1 p1' /\ loc_includes p2 p2' /\ loc_disjoint p1 p2))
   (ensures (loc_disjoint p1' p2')) =
-  admit()
+  ()
 
 let loc_disjoint_aloc_intro
   (#aloc: Type) (#c: cls aloc)
@@ -171,7 +178,7 @@ let loc_disjoint_aloc_intro
 : Lemma
   (requires (c.aloc_disjoint b1 b2))
   (ensures (loc_disjoint (loc_of_aloc b1) (loc_of_aloc #_ #c b2))) =
-  admit()
+  Classical.forall_intro_4 (fun x y z -> Classical.move_requires (c.aloc_disjoint_includes x y z))
 
 let loc_includes_disjoint_elim
   #al (c: cls al)
@@ -205,35 +212,35 @@ let loc_union_idem
   (s: loc c)
 : Lemma
   (loc_union s s == s) =
-  admit()
+  assert (loc_union s s `GSet.equal` s)
 
 let loc_union_comm
   (#aloc: Type) (#c: cls aloc)
   (s1 s2: loc c)
 : Lemma
   (loc_union s1 s2 == loc_union s2 s1) =
-  admit()
+  assert (loc_union s1 s2 `GSet.equal` loc_union s2 s1)
 
 let loc_union_assoc
   (#aloc: Type) (#c: cls aloc)
   (s1 s2 s3: loc c)
 : Lemma
   (loc_union s1 (loc_union s2 s3) == loc_union (loc_union s1 s2) s3) =
-  admit()
+  assert (loc_union s1 (loc_union s2 s3) `GSet.equal` loc_union (loc_union s1 s2) s3)
 
 let loc_union_loc_none_l
   (#aloc: Type) (#c: cls aloc)
   (s: loc c)
 : Lemma
   (loc_union loc_none s == s) =
-  admit()
+  assert (loc_union loc_none s `GSet.equal` s)
 
 let loc_union_loc_none_r
   (#aloc: Type) (#c: cls aloc)
   (s: loc c)
 : Lemma
   (loc_union s loc_none == s) =
-  admit()
+  assert (loc_union s loc_none `GSet.equal` s)
 
 let preserved #al (#c: cls al) (l: loc c) (h1 h2: HS.mem) : GTot Type0 =
   forall (x: al) . {:pattern (x `GSet.mem` l)} x `GSet.mem` l ==> c.aloc_preserved x h1 h2
@@ -254,7 +261,7 @@ let loc_includes_refl
   (s: loc c)
 : Lemma
   (loc_includes s s) =
-  admit()
+  Classical.forall_intro c.aloc_includes_refl
 
 let loc_includes_trans
   (#aloc: Type) (#c: cls aloc)
@@ -262,7 +269,7 @@ let loc_includes_trans
 : Lemma
   (requires (loc_includes s1 s2 /\ loc_includes s2 s3))
   (ensures (loc_includes s1 s3)) =
-  admit()
+  Classical.forall_intro_3 (fun x y -> Classical.move_requires (c.aloc_includes_trans x y))
 
 let loc_includes_union_r
   (#aloc: Type) (#c: cls aloc)
@@ -270,7 +277,7 @@ let loc_includes_union_r
 : Lemma
   (requires (loc_includes s s1 /\ loc_includes s s2))
   (ensures (loc_includes s (loc_union s1 s2))) =
-  admit()
+  ()
 
 let loc_includes_union_l
   (#aloc: Type) (#c: cls aloc)
@@ -278,14 +285,18 @@ let loc_includes_union_l
 : Lemma
   (requires (loc_includes s1 s \/ loc_includes s2 s))
   (ensures (loc_includes (loc_union s1 s2) s)) =
-  admit()
+  Classical.forall_intro c.aloc_includes_refl;
+  assert (forall x . x `GSet.mem` s1 ==> x `GSet.mem` (loc_union s1 s2));
+  assert (forall x . x `GSet.mem` s2 ==> x `GSet.mem` (loc_union s1 s2));
+  Classical.move_requires (loc_includes_trans (loc_union s1 s2) s1) s;
+  Classical.move_requires (loc_includes_trans (loc_union s1 s2) s2) s
 
 let loc_includes_none
   (#aloc: Type) (#c: cls aloc)
   (s: loc c)
 : Lemma
   (loc_includes s loc_none) =
-  admit()
+  ()
 
 let loc_includes_none_elim
   (#aloc: Type) (#c: cls aloc)
@@ -293,7 +304,7 @@ let loc_includes_none_elim
 : Lemma
   (requires (loc_includes loc_none s))
   (ensures (s == loc_none)) =
-  admit()
+  assert (s `GSet.equal` loc_none #_ #c)
 
 
 let modifies_aloc_elim
@@ -309,7 +320,8 @@ let modifies_aloc_elim
   (ensures (
     c.aloc_preserved b h h'
   )) =
-  admit()
+  Classical.forall_intro c.aloc_includes_refl;
+  assert (b `GSet.mem` (loc_of_aloc #_ #c b))
 
 let modifies_refl
   (#aloc: Type) (#c: cls aloc)
@@ -317,7 +329,7 @@ let modifies_refl
   (h: HS.mem)
 : Lemma
   (modifies s h h) =
-  admit()
+  Classical.forall_intro_2 c.aloc_preserved_refl
 
 
 let modifies_loc_includes
@@ -328,7 +340,8 @@ let modifies_loc_includes
 : Lemma
   (requires (modifies s2 h h' /\ loc_includes s1 s2))
   (ensures (modifies s1 h h')) =
-  admit()
+  Classical.forall_intro (loc_includes_refl #_ #c);
+  Classical.forall_intro_4 (fun x y z -> Classical.move_requires (loc_disjoint_includes #_ #c x y z))
 
 
 let modifies_trans
@@ -340,11 +353,62 @@ let modifies_trans
 : Lemma
   (requires (modifies s12 h1 h2 /\ modifies s23 h2 h3))
   (ensures (modifies (loc_union s12 s23) h1 h3)) =
-  admit()
+  loc_includes_refl s12;
+  loc_includes_union_l s12 s23 s12;
+  modifies_loc_includes (loc_union s12 s23) h1 h2 s12;
+  loc_includes_refl s23;
+  loc_includes_union_l s12 s23 s23;
+  modifies_loc_includes (loc_union s12 s23) h2 h3 s23;
+  Classical.forall_intro_4 (fun x y z -> Classical.move_requires (c.aloc_preserved_trans x y z))
 
 let loc_unused_in_used_in_disjoint (#al: Type) (c: cls al) (h: HS.mem) : Lemma
   (loc_unused_in c h `loc_disjoint` loc_used_in c h) =
-  admit()
+  Classical.forall_intro_3 c.aloc_used_in_unused_in_disjoint
+
+let modifies_aloc_intro'
+  (#al: Type) (#c: cls al) (l: loc c) (h h' : HS.mem)
+  (alocs: (
+    (x: al) ->
+    Lemma
+    (requires (loc_disjoint l (loc_of_aloc x)))
+    (ensures (c.aloc_preserved x h h'))
+  ))
+: Lemma
+  (modifies l h h')
+= 
+  let f
+    (l': loc c)
+  : Lemma
+    (requires (l' `loc_disjoint` l))
+    (ensures (preserved l' h h'))
+  = let g
+      (x: al)
+    : Lemma
+      (requires (x `GSet.mem` l'))
+      (ensures (c.aloc_preserved x h h'))
+    = alocs x
+    in
+    Classical.forall_intro (Classical.move_requires g)
+  in
+  Classical.forall_intro (Classical.move_requires f)
+
+let modifies_aloc_intro
+  (#al: Type) (#c: cls al) (z: al) (h h' : HS.mem)
+  (alocs: (
+    (x: al) ->
+    Lemma
+    (requires (c.aloc_disjoint x z))
+    (ensures (c.aloc_preserved x h h'))
+  ))
+: Lemma
+  (modifies (loc_of_aloc #_ #c z) h h') =
+  modifies_aloc_intro' #_ #c (loc_of_aloc z) h h' (fun x ->
+    c.aloc_includes_refl z;
+    assert (z `GSet.mem` loc_of_aloc #_ #c z);
+    c.aloc_includes_refl x;
+    assert (x `GSet.mem` loc_of_aloc #_ #c x);
+    alocs x
+  )
 
 let modifies_only_used_in
   (#al: Type)
@@ -354,7 +418,28 @@ let modifies_only_used_in
 : Lemma
   (requires (modifies (loc_unused_in c h `loc_union` l) h h'))
   (ensures (modifies l h h')) =
-  admit()
+  modifies_aloc_intro' l h h' (fun x ->
+    c.aloc_used_in_or_unused_in x h;
+    Classical.forall_intro_2 (fun x y -> c.aloc_used_in_unused_in_disjoint x y h);
+    Classical.forall_intro c.aloc_includes_refl;
+    c.aloc_disjoint_not_includes x x;
+    if StrongExcludedMiddle.strong_excluded_middle (x `c.aloc_used_in` h) then begin
+      let f
+        (x' y' : al)
+      : Lemma
+        (requires (x `c.aloc_includes` x' /\ y' `c.aloc_unused_in` h))
+        (ensures (y' `c.aloc_disjoint` x'))
+      = c.aloc_disjoint_sym x y' ;
+        c.aloc_disjoint_includes y' x y' x'
+      in
+      Classical.forall_intro_2 (fun x -> Classical.move_requires (f x));
+      assert (loc_unused_in c h `loc_disjoint` loc_of_aloc x);
+      assert ((loc_unused_in c h `loc_union` l) `loc_disjoint` loc_of_aloc x);
+      assert (x `GSet.mem` loc_of_aloc #_ #c x)
+    end else begin
+      c.aloc_unused_in_preserved x h h'
+    end
+  )
 
 let modifies_loc_unused_in
   #al
@@ -374,16 +459,12 @@ let aloc_unused_in_intro #al (c: cls al) (l: al) (h: HS.mem) : Lemma
   (requires (l `c.aloc_unused_in` h))
   (ensures (loc_unused_in c h `loc_includes` loc_of_aloc l))
   =
-  admit()
-
-let modifies_aloc_intro
-  (#al: Type) (#c: cls al) (z: al) (h h' : HS.mem)
-  (alocs: (
-    (x: al) ->
-    Lemma
-    (requires (c.aloc_disjoint x z))
-    (ensures (c.aloc_preserved x h h'))
-  ))
-: Lemma
-  (modifies (loc_of_aloc #_ #c z) h h') =
-  admit()
+  let f
+    (x: al)
+  : Lemma
+    (requires (l `c.aloc_includes` x))
+    (ensures (x `GSet.mem` loc_unused_in c h))
+  = c.aloc_unused_in_includes l x h
+  in
+  Classical.forall_intro (Classical.move_requires f);
+  Classical.forall_intro c.aloc_includes_refl
